examples/lrat_checker/parsingScript.sml
@@ -1,0 +1,224 @@
+(*
+   Parsing interface for DIMACS and LRAT
+*)
+open preamble miscTheory lratTheory mlintTheory;
+
+val _ = new_theory "parsing";
+
+(*
+  Parses a list of strings (1 per line of a file) in DIMACS format
+*)
+
+val blanks_def = Define`
+  blanks (c:char) ⇔ c = #" " ∨ c = #"\n" ∨ c = #"\t"`
+
+(* A clause line must end with 0,
+  cannot contain 0s elsewhere, and is within the var bound *)
+val parse_clause_def = Define`
+  (parse_clause maxvar [] (acc:clause) = NONE) ∧
+  (parse_clause maxvar [c] acc =
+    if c = (strlit "0") then SOME acc
+    else NONE) ∧
+  (parse_clause maxvar (x::xs) acc =
+    case mlint$fromString x of
+      NONE => NONE
+    | SOME l =>
+    if l = 0 ∨ l > &maxvar ∨ l < -&maxvar then NONE
+    else parse_clause maxvar xs (l::acc)
+  )`
+
+(* A single line of file as a string *)
+(* val parse_dimacs_line_def = Define`
+  (parse_dimacs_line maxvar str =
+  (* For now, split the line into space separated string*)
+  let ls = tokens blanks str in parse_clause maxvar ls [])` *)
+
+val parse_header_line_def = Define`
+  parse_header_line str =
+  let ls = tokens blanks str in
+  case ls of
+    [p; cnf; vars; numcls] =>
+    if p = strlit "p" ∧ cnf = strlit "cnf"
+    then
+      case (mlint$fromNatString vars, mlint$fromNatString numcls)
+      of
+        (SOME v,SOME c) => SOME (v,c)
+      | _ => NONE
+    else NONE
+  | _ => NONE`
+
+(*
+val res = EVAL ``parse_header_line (strlit"p cnf 1 2")``
+*)
+
+(*
+  parse a strings as DIMACS
+  TODO: this should be replaced with TextIO version
+*)
+val build_fml_def = Define`
+  (build_fml maxvar (id:num) [] (acc:int list spt) = SOME acc) ∧
+  (build_fml maxvar id (s::ss) acc =
+    case parse_clause maxvar s [] of
+    NONE => NONE
+  | SOME cl => build_fml maxvar (id+1) ss (insert id cl acc))`
+
+val parse_dimacs_def = Define`
+  parse_dimacs strs =
+  case strs of
+    s::ss =>
+      (case parse_header_line s of
+      SOME (vars,clauses) =>
+        let tokss = MAP (tokens blanks) ss in
+        let nocomments = FILTER (λs. case s of x::xs => x ≠ strlit "c" | [] => T) tokss in
+        if LENGTH nocomments = clauses then
+          build_fml vars 1 nocomments LN
+        else NONE
+      | NONE => NONE)
+  | [] => NONE`
+
+Theorem parse_clause_wf:
+  ∀v ls acc.
+  wf_clause acc ∧
+  parse_clause v ls acc = SOME res ⇒
+  wf_clause res
+Proof
+  ho_match_mp_tac (fetch "-" "parse_clause_ind")>>fs[parse_clause_def]>>
+  rw[]>> every_case_tac>>fs[]>>
+  rfs[wf_clause_def]
+QED
+
+Theorem build_fml_wf:
+  ∀ls acc i.
+  wf_fml acc ∧
+  build_fml v i ls acc = SOME acc' ⇒
+  wf_fml acc'
+Proof
+  Induct>>fs[build_fml_def]>>
+  rw[]>>every_case_tac>>fs[]>>
+  first_x_assum match_mp_tac>>
+  qexists_tac`insert i x acc`>>
+  qexists_tac`i+1`>>
+  simp[]>>
+  match_mp_tac wf_fml_insert>>
+  `wf_clause []` by fs[wf_clause_def]>>
+  metis_tac[parse_clause_wf]
+QED
+
+(* Parse everything until the next zero and returns it *)
+val parse_until_zero_def = Define`
+  (parse_until_zero [] acc = NONE) ∧
+  (parse_until_zero (x::xs) acc =
+    case mlint$fromString x of
+      NONE => NONE
+    | SOME l =>
+    if l = 0:int then
+      SOME (REVERSE acc, xs)
+    else
+      parse_until_zero xs (l::acc)
+  )`
+
+(* Parse everything until the next non-positive and returns it *)
+val parse_until_nn_def = Define`
+  (parse_until_nn [] acc = NONE) ∧
+  (parse_until_nn (x::xs) acc =
+    case mlint$fromString x of
+      NONE => NONE
+    | SOME l =>
+    if l ≤ 0:int then
+      SOME (Num (-l), REVERSE acc, xs)
+    else
+      parse_until_nn xs (Num l::acc)
+  )`
+
+val parse_until_nn_length = Q.prove(`
+  ∀ls acc a b c.
+  parse_until_nn ls acc = SOME(a,b,c) ⇒
+  LENGTH c < LENGTH ls`,
+  Induct>>fs[parse_until_nn_def]>>
+  rw[]>>every_case_tac>>fs[]>>
+  first_x_assum drule>>
+  fs[]
+QED
+
+val parse_RAT_hint_def = tDefine "parse_RAT_hint" `
+  parse_RAT_hint id xs acc =
+  if id = 0 then
+    if xs = [] then SOME acc
+    else NONE
+  else
+  case parse_until_nn xs [] of
+    NONE => NONE
+  | SOME (n,clause,rest) =>
+      parse_RAT_hint n rest (insert id clause acc)`
+  (WF_REL_TAC `measure (LENGTH o (FST o SND))`>>
+  rw[]>>
+  drule parse_until_nn_length>>fs[])
+
+(* LRAT parser *)
+val parse_lratstep_def = Define`
+  (parse_lratstep (cid::first::rest) =
+  if first = strlit "d" then
+    (* deletion line *)
+    (case parse_until_nn rest [] of
+       SOME (n, ls, []) => if n = 0 then SOME (Delete ls) else NONE
+      | _ => NONE)
+  else
+  case mlint$fromNatString cid of
+    NONE => NONE
+  | SOME cid =>
+    (* RAT line *)
+    case parse_until_zero (first::rest) [] of
+      NONE => NONE
+    | SOME (clause,rest) =>
+      case parse_until_nn rest [] of
+        NONE => NONE
+      | SOME (id,hint,rest) =>
+        case parse_RAT_hint id rest LN of
+          NONE => NONE
+        | SOME sp => SOME (RAT cid clause hint sp)
+  )`
+
+val parse_lrat_aux_def = Define`
+  (parse_lrat_aux [] acc = SOME (REVERSE acc)) ∧
+  (parse_lrat_aux (l::ls) acc =
+    case parse_lratstep (tokens blanks l) of
+      NONE => NONE
+    | SOME step => parse_lrat_aux ls (step::acc)
+    )`
+
+val parse_lrat_def = Define`
+  parse_lrat ls = parse_lrat_aux ls []`
+
+val dimacsraw = ``[
+  strlit "p cnf 5 8 ";
+  strlit "    1  4 0";
+  strlit "    1  5 0";
+  strlit "    2  4 0";
+  strlit "    2  5 0";
+  strlit "    3  4 0";
+  strlit "    3  5 0";
+  strlit "-1 -2 -3 0";
+  strlit "   -4 -5 0";
+  ]``;
+
+val cnf = rconc (EVAL ``THE (parse_dimacs ^(dimacsraw))``);
+
+val lratraw = ``[
+  strlit"8 d 0";
+  strlit"9 6 1 0 1 2 8 0";
+  strlit"10 6 2 0 3 4 8 0";
+  strlit"11 6 3 0 5 6 8 0";
+  strlit"12 -6 4 0 1 5 7 3 0";
+  strlit"12 d 1 5 3 0";
+  strlit"13 -6 5 0 2 6 7 4 0";
+  strlit"13 d 2 6 4 0";
+  strlit"14 6 0 9 10 11 7 0";
+  strlit"14 d 9 10 11 7 0";
+  strlit"16 0 14 12 13 8 0";
+  ]``;
+
+val lrat = rconc (EVAL ``THE (parse_lrat ^(lratraw))``);
+
+val check = EVAL``check_lrat ^(lrat) ^(cnf)``;
+
+val _ = export_theory ();
