examples/lrat_checker/README.md
@@ -1,0 +1,7 @@
+An LRAT checker built on CakeML
+
+[lratScript.sml](lratScript.sml):
+Verification of LRAT checker
+
+[ramseyScript.sml](ramseyScript.sml):
+Defining the Ramsey number and SAT encoding
